YLM: implemented fourth protocol step
aead and event pred are still hard coded as True and need to be redefined in
order to be able to pass on statements about the key secrecy to the responder.

yahalom/YLM.Protocol.fst
@@ -160,6 +160,13 @@ let server_send_msg_3 srv msg2_idx =
           publishable_readers_implies_corruption #now [P b; P srv];
           readers_is_injective_2 b srv;
           assert(corrupt_id now (P b) \/ corrupt_id now (P srv) \/ did_event_occur_before now b (event_req_key a b srv n_a n_b));
+          aead_dec_plaintext_publishable_if_key_and_ciphertext_publishable_forall ylm_global_usage;
+          assert(is_publishable ylm_global_usage now ser_ev_b \/ aead_pred ylm_usage_preds now "YLM.lt_key" k_bs ser_ev_b ad);
+          splittable_term_publishable_implies_components_publishable_forall ylm_global_usage;
+          assert(is_publishable ylm_global_usage now n_a /\ is_publishable ylm_global_usage now n_b
+            \/ aead_pred ylm_usage_preds now "YLM.lt_key" k_bs ser_ev_b ad);
+          assert(is_publishable ylm_global_usage now n_a /\ is_publishable ylm_global_usage now n_b
+            \/ did_event_occur_before now b (event_req_key a b srv n_a n_b));
           let prev = now in
           let event = event_send_key a b srv n_a n_b k_ab in
           trigger_event #ylm_preds srv event;
@@ -167,13 +174,6 @@ let server_send_msg_3 srv msg2_idx =
           // create and send third message
           let ev3_i = EncMsg3_I b k_ab n_a n_b in
           let now = global_timestamp () in
-          aead_dec_plaintext_publishable_if_key_and_ciphertext_publishable_forall ylm_global_usage;
-          assert(is_publishable ylm_global_usage prev ser_ev_b \/ aead_pred ylm_usage_preds prev "YLM.lt_key" k_bs ser_ev_b ad);
-          splittable_term_publishable_implies_components_publishable_forall ylm_global_usage;
-          assert(is_publishable ylm_global_usage prev n_a /\ is_publishable ylm_global_usage prev n_b
-            \/ aead_pred ylm_usage_preds prev "YLM.lt_key" k_bs ser_ev_b ad);
-          assert(is_publishable ylm_global_usage prev n_a /\ is_publishable ylm_global_usage prev n_b
-            \/ did_event_occur_before prev b (event_req_key a b srv n_a n_b));
           can_flow_later_forall cpred (get_label ylm_key_usages n_a) public;
           rand_is_secret #ylm_global_usage #now #(readers [P b; P a; P srv]) #(nonce_usage "YLM.nonce_b") n_b;
           assert(is_msg ylm_global_usage now n_a public /\ is_publishable ylm_global_usage now n_b \/ is_secret ylm_global_usage now n_b (readers [P b; P a; P srv]) (nonce_usage "YLM.nonce_b"));
@@ -213,4 +213,91 @@ let server_send_msg_3 srv msg2_idx =
     else error "[srv_send_m3] actual responder does not match with responder in second message"
   )
   | _ -> error "[srv_send_m3] wrong message"
+
+let initiator_send_msg_4 a kas_idx msg3_idx a_si =
+  // get initiator session
+  let now = global_timestamp () in
+  let (|a_vi,ser_st|) = get_session #ylm_preds #now a a_si in
+
+  match parse_session_st ser_st with
+  | Success (InitiatorSentMsg1 b n_a) -> (
+    // receive and parse third message
+    let (|_,srv,ser_msg3|) = receive_i #ylm_preds msg3_idx a in
+
+    match parse_msg ser_msg3 with
+    | Success (Msg3 c_ev_a c_ev_b) -> (
+      // get initiator long term key
+      let (|_,(PKeySession srv' k_as)|) = get_lt_key_session a kas_idx in
+
+      if srv = srv' then
+        // decrypt part of third message encrypted by server for initiator
+        let iv = string_to_bytes #ylm_global_usage #now "iv" in
+        let ad = string_to_bytes #ylm_global_usage #now "ev3_i" in
+        match aead_dec #ylm_global_usage #now #(get_label ylm_key_usages k_as) k_as iv c_ev_a ad with
+        | Success ser_ev_a -> (
+          match parse_encval ser_ev_a with
+          | Success (EncMsg3_I b' k_ab n_a' n_b) -> (
+            if b = b' && n_a = n_a' then
+              // trigger event 'fwd key'
+              let prev = now in
+              let event = event_fwd_key a b srv n_a n_b k_ab in
+              trigger_event #ylm_preds a event;
+
+              // create and send fourth message
+              let ev4 = EncMsg4 n_b in
+              let now = global_timestamp () in
+              assert(is_publishable ylm_global_usage prev k_as \/ aead_pred ylm_usage_preds prev "YLM.lt_key" k_as ser_ev_a ad);
+              aead_dec_plaintext_publishable_if_key_and_ciphertext_publishable_forall ylm_global_usage;
+              assert(is_publishable ylm_global_usage prev ser_ev_a \/ aead_pred ylm_usage_preds prev "YLM.lt_key" k_as ser_ev_a ad);
+              splittable_term_publishable_implies_components_publishable_forall ylm_global_usage;
+              assert(is_publishable ylm_global_usage prev n_b \/ aead_pred ylm_usage_preds prev "YLM.lt_key" k_as ser_ev_a ad);
+              readers_is_injective_2 a srv;
+              assert(is_publishable ylm_global_usage prev n_b \/ did_event_occur_before prev srv (event_send_key a b srv n_a n_b k_ab));
+              assert(is_publishable ylm_global_usage prev n_b
+                \/ was_rand_generated_before prev k_ab (readers [P srv; P a; P b]) (aead_usage "YLM.comm_key")
+                /\ did_event_occur_before prev b (event_req_key a b srv n_a n_b));
+              can_flow_later_forall cpred (get_label ylm_key_usages n_b) public;
+              rand_is_secret #ylm_global_usage #now #(readers [P srv; P a; P b]) #(aead_usage "YLM.comm_key") k_ab;
+              rand_is_secret #ylm_global_usage #now #(readers [P b; P a; P srv]) #(nonce_usage "YLM.nonce_b") n_b;
+              assert(is_msg ylm_global_usage now n_b public
+                \/ is_secret ylm_global_usage now k_ab (readers [P srv; P a; P b]) (aead_usage "YLM.comm_key")
+                /\ is_secret ylm_global_usage now n_b (readers [P b; P a; P srv]) (nonce_usage "YLM.nonce_b"));
+              flows_to_public_can_flow now (get_label ylm_key_usages n_b) (get_label ylm_key_usages k_ab);
+              includes_can_flow_lemma now [P b; P a; P srv] [P srv; P a; P b];
+              let ser_ev4 = serialize_encval now ev4 (get_label ylm_key_usages k_ab) in
+              let ad = string_to_bytes #ylm_global_usage #now "ev4" in
+              parse_serialize_encval_lemma now ev4 (get_label ylm_key_usages k_ab);
+              let c_ev4 = aead_enc #ylm_global_usage #now #(get_label ylm_key_usages k_ab) k_ab iv ser_ev4 ad in
+
+              let c_ev_b:msg ylm_global_usage now public = c_ev_b in
+              let msg4 = Msg4 c_ev_b c_ev4 in
+              let ser_msg4 = serialize_msg now msg4 in
+
+              let msg4_idx = send #ylm_preds #now a b ser_msg4 in
+
+              // update initiator session
+              let st_i_sent_m4 = InitiatorSentMsg4 b srv k_ab in
+              let now = global_timestamp () in
+              assert(is_publishable ylm_global_usage prev k_as \/ did_event_occur_before prev srv (event_send_key a b srv n_a n_b k_ab));
+              includes_corrupt_2_lemma prev (P a) (P srv);
+              publishable_readers_implies_corruption #now [P a; P srv];
+              assert(corrupt_id prev (P a) \/ corrupt_id prev (P srv) \/ did_event_occur_before prev srv (event_send_key a b srv n_a n_b k_ab));
+              assert(corrupt_id prev (P a) \/ corrupt_id prev (P srv)
+                \/ was_rand_generated_before prev k_ab (readers [P srv; P a; P b]) (aead_usage "YLM.comm_key"));
+              includes_can_flow_lemma now [P srv; P a; P b] [P a];
+              let ser_st = serialize_session_st now a a_si a_vi st_i_sent_m4 in
+
+              update_session #ylm_preds #now a a_si a_vi ser_st;
+
+              msg4_idx
+            else error "[i_send_m4] responder or nonce mismatch in initiator encval"
+          )
+          | _ -> error "[i_send_m4] wrong initiator encval"
+        )
+        | Error e -> error ("[i_send_m4] " ^ e)
+      else error "[i_send_m4] actual server does not match with server of long term key session"
+    )
+    | _ -> error "[i_send_m4] wrong message"
+  )
+  | _ -> error "[i_send_m4] wrong session"
 #pop-options
