yahalom/YLM.Sessions.fsti
@@ -40,7 +40,7 @@ let valid_session (i:nat) (p:principal) (si vi:nat) (st:session_st) =
   | AuthServerSentMsg3 a b k_ab -> is_comm_key i k_ab p a b
   | InitiatorSentMsg4 b srv k_ab ->
     M.is_msg i k_ab (readers [P p]) /\
-    (is_labeled i k_ab (readers [P srv; P p; P b]) \/ LC.corrupt_id i (P srv) \/ LC.corrupt_id i (P p) \/ LC.corrupt_id i (P b))
+    (is_labeled i k_ab (readers [P srv; P p; P b]) \/ LC.corrupt_id i (P srv) \/ LC.corrupt_id i (P p))
   | ResponderRecvedMsg4 a srv k_ab ->
     M.is_msg i k_ab (readers [P p]) /\
     (is_labeled i k_ab (readers [P srv; P a; P p]) \/ LC.corrupt_id i (P srv) \/ LC.corrupt_id i (P a) \/ LC.corrupt_id i (P p))
@@ -77,7 +77,14 @@ let epred idx s e =
       srv = s /\
       was_rand_generated_before idx k_ab (readers [P srv; P a; P b]) (aead_usage "YLM.comm_key") /\
       (did_event_occur_before idx b (M.event_req_key a b srv n_a n_b) \/
-      LC.corrupt_id idx (P b) \/ LC.corrupt_id idx (P srv))
+      (LC.corrupt_id idx (P b) \/ LC.corrupt_id idx (P srv)) /\ M.is_msg idx n_b public)
+    | _ -> False
+  )
+  | ("fwd_key",[a_bytes;b_bytes;srv_bytes;n_a;n_b;k_ab]) -> (
+    match (bytes_to_string a_bytes, bytes_to_string b_bytes, bytes_to_string srv_bytes) with
+    | (Success a, Success b, Success srv) ->
+      a = s /\
+      True
     | _ -> False
   )
   | _ -> False
